SkLean/LcSkmEtaUntyped.lean
@@ -1,0 +1,177 @@
+/-
+# Synthesizing Expressions with \\(\eta\\)-Reduction
+
+In the previous chapter, we saw that we can create an expression representing the nondependent \\(\rightarrow\\) type. However, \\(K\\) and \\(S\\) are dependent. I make use of a translation algorithm to generate point-free expressions involving only \\(S\\), \\(K\\), and \\(M\\) for these expressions.
+
+## Syntax Tree
+
+As outlined prior, our core language consists only of the objects \\(S\\), \\(K\\), \\(M\\), and \\(\text{Type}_{n}\\). I define the syntax-tree in Lean as such:
+-/
+
+import Mathlib.Tactic
+import SkLean.Ast3
+
+namespace Expr
+
+def toStringImpl (e : Expr) : String :=
+  match e with
+    | .k          => "K"
+    | .s          => "S"
+    | .m          => "M"
+    | .call e₁ e₂ => s!"({toStringImpl e₁} {toStringImpl e₂})"
+
+end Expr
+
+instance : ToString Expr where
+  toString := fun e => e.toStringImpl
+
+  /-
+For translation purposes, I define an AST for the (optionally) simply-typed \\(\lambda\\)-calculus, extended with our syntax tree. I use de bruijn indices to refer to variables.
+-/
+
+inductive LExpr where
+  | var   : ℕ     → LExpr
+  | call  : LExpr → LExpr → LExpr
+  | raw   : Expr  → LExpr
+  | lam   : LExpr → LExpr
+  | m     : LExpr
+  | s     : LExpr
+  | k     : LExpr
+deriving Repr
+
+namespace LExpr
+
+def toStringImpl (e : LExpr) : String :=
+  match e with
+    | .var n            => s!"var {n}"
+    | .raw e            => s!"{e}"
+    | .call e₁ e₂       => s!"({e₁.toStringImpl} {e₂.toStringImpl})"
+    | .lam body       => s!"λ {body.toStringImpl}"
+    | .m                => "M"
+    | .k                => "K"
+    | .s                => "S"
+
+end LExpr
+
+instance : ToString LExpr where
+  toString := fun e => e.toStringImpl
+
+namespace Expr
+
+def dec_vars (depth : ℕ) (e : LExpr) : LExpr :=
+  match e with
+    | .var n =>
+      if n > depth then
+        .var n.pred
+      else
+        .var n
+    | .call lhs rhs => .call (dec_vars depth lhs) (dec_vars depth rhs)
+    | .lam body => .lam (dec_vars depth.succ body)
+    | x => x
+
+-- To eliminate λ-abstraction as much as possible
+-- This function abstracts variable 0 from a lambda-free body.
+partial def lift (e : LExpr) : LExpr :=
+  -- We shouldn't really do anything unless
+  -- the expression is a lambda abstraction
+  -- In the case of e₁ e₂ application,
+  -- we must lift both e₁ and e₂ first,
+  -- then apply the S-transformation
+  -- In the case of lambda abstraction with (.var 0)
+  -- as the body, apply the I-transformation
+  -- In the case of lambda abstraction with
+  -- any other variable which is not free
+  -- we decrement the index, since
+  -- one abstraction has been removed
+  let e' := match e with
+    | .call lhs rhs =>
+      (.call (lift lhs) (lift rhs))
+    | .lam (.call lhs rhs) =>
+      let lhs' := lift lhs |> LExpr.lam
+      let rhs' := lift rhs |> LExpr.lam
+
+      lift (.call (.call .s lhs') rhs')
+    | .lam (.var 0) =>
+      (.call (.call .s .k) .k)
+    | .lam (.lam x') =>
+      let body' := lift (.lam x')
+
+      lift (.lam body')
+    | .lam x =>
+      let x' := lift x |> dec_vars 0
+
+      lift (.call .k x')
+    | e => e
+
+    e'
+
+def to_sk (e : LExpr) : Option Expr :=
+  match e with
+    | .call lhs rhs => do
+      SKM[(#(← to_sk lhs) #(← to_sk rhs))]
+    | .k => SKM[K]
+    | .s => SKM[S]
+    | .m => SKM[M]
+    | .raw e => e
+    | _ => none
+
+def to_sk_unsafe (e : LExpr) : Expr :=
+  match e with
+    | .call lhs rhs =>
+      SKM[(#(to_sk_unsafe lhs) #(to_sk_unsafe rhs))]
+    | .k => SKM[K]
+    | .s => SKM[S]
+    | .m => SKM[M]
+    | .raw e => e
+    | _ => SKM[K]
+
+/-
+We can now define the \\(\rightarrow\\) expression using our \\(\lambda\\)-calculus AST and translate to \\(SK(M)\\) using our `lift` and `to_sk` functions. Note that since universes are stratified, \\(\rightarrow\\) is polymorphic at the meta level to universe levels. In practice, the compiler generates an \\(\rightarrow\\) expression for all universes used in the program. Furthermore, universes above \\(1\\) are rarely used.
+-/
+
+def arrow_lc : LExpr := (.lam (.lam (.call (.call (.call .k (.call .m (.var 0))) (.var 1)) (.var 0))))
+
+/-
+For testing purposes, we will write `partial` evaluation and typing functions:
+-/
+
+def eval_n (n : ℕ) (e : Expr) : Expr :=
+  if n = 0 then
+    e
+ else
+   let e' := match e with
+     | SKM[((((K _α) _β) x) _y)] => x
+     | SKM[((((((S _α) _β) _γ) x) y) z)] => SKM[((x z) (y z))]
+     | SKM[(lhs rhs)] =>
+       SKM[((#(eval_n n.pred lhs)) #(eval_n n.pred.pred rhs))]
+     | x => x
+
+   eval_n n.pred.pred.pred e'
+
+-- Type of K : λ α.→ (M α) (λ β.(→ (M β)) (M α))
+def t_k := (.lam (.call (.call (.raw arrow) (.call .m (.var 0))) (.lam (.call (.call (.raw arrow) (.call .m (.var 0))) (.call .m (.var 1))))))
+  |> lift
+  |> to_sk_unsafe
+
+-- Type of M: λ e. → (M e) (M (M e))
+def t_m := (.lam (.call (.call (.raw arrow) (.call .m (.var 0))) (.call .m (.call .m (.var 0)))))
+  |> lift
+  |> to_sk_unsafe
+
+-- Type of S : λ α.→ (M α) (λ β.→ (M β) (λ γ.→ (M γ) (snd ((snd ((M α) γ)) (snd ((M β) γ))))))
+def t_s := (.lam
+  (.call
+    (.call (.raw arrow) (.call .m (.var 0)))
+    (.lam
+      (.call
+        (.call (.raw arrow) (.call .m (.var 0)))
+        (.lam
+          (.call
+            (.call (.raw arrow) (.call .m (.var 0)))
+            (.call (.raw t_out) (.call (.call (.raw t_out) (.call (.call .m (.var 2)) (.var 0))) (.call (.raw t_out) (.call (.call .m (.var 1)) (.var 0)))))))))))
+  |> lift
+  |> to_sk_unsafe
+
+#eval s!"{t_k}"
+#eval s!"{t_s}"
+#eval s!"{t_m}"
